src/SDK/Keyring/KMSKeyring.dfy
@@ -18,7 +18,10 @@ module {:extern "KMSKeyringDef"} KMSKeyringDef {
   import UTF8
 
   // UTF-8 encoded "aws-kms"
-  const PROVIDER_ID: UTF8.ValidUTF8Bytes := [0x61, 0x77, 0x73, 0x2D, 0x6B, 0x6D, 0x73];
+  const PROVIDER_ID: UTF8.ValidUTF8Bytes :=
+    var s := [0x61, 0x77, 0x73, 0x2D, 0x6B, 0x6D, 0x73];
+    assert UTF8.ValidUTF8Range(s, 0, 7);
+    s
 
   function method RegionFromKMSKeyARN(arn: KMSUtils.CustomerMasterKey): Result<string>
   {
